source/consistent.v
@@ -1,0 +1,86 @@
+
+From S5 Require Export soundness.
+
+Definition consistent (G : Form -> Prop) : Prop :=
+  ~(ax_s5 G F_).
+
+Lemma consistent_xor (G : Form -> Prop) (x : Form) :
+  consistent G -> ~(ax_s5 G x /\ ax_s5 G (Neg x)).
+Proof.
+  intros H0 [H1 H2]. apply H0. unfold Neg in H2. eapply mp.
+  - apply H2.
+  - assumption.
+Qed.
+
+Lemma consistent_subset (F G : Form -> Prop) :
+  subset F G /\ consistent G -> consistent F.
+Proof.
+  intros [Hs Hcon] Hf. unfold consistent, not in Hcon. apply Hcon.
+  eapply ax_s5_subset.
+  - apply Hf.
+  - assumption. 
+Qed.
+
+Lemma deduce_not_consistent_add_neg_singleton (G : Form -> Prop) (x : Form) :
+  consistent G /\ ax_s5 G x -> ~consistent (add_singleton G (Neg x)).
+Proof.
+  intros [H0 H1] H2. eapply consistent_xor.
+  - apply H2.
+  - split.
+    + eapply ax_s5_subset.
+      * apply H1.
+      * apply subset_add_singleton. 
+    + apply a_0. apply member_add_singleton.
+Qed.
+
+Lemma consistent_add_singleton_not_deduce (G : Form -> Prop) (x : Form) :
+  consistent (add_singleton G x) -> ~ax_s5 G (Neg x).
+Proof.
+  intros H0 H1. eapply consistent_xor.
+  - apply H0.
+  - split.
+    + apply a_0. apply member_add_singleton.
+    + eapply ax_s5_subset.
+      * apply H1.
+      * apply subset_add_singleton.
+Qed.
+
+Lemma inconsistent_consistent (G : Form -> Prop) (x : Form) : 
+  consistent G -> 
+  ~ consistent (add_singleton G x) -> consistent (add_singleton G (Neg x)).
+Proof.
+  intros HG H1 H2. assert (H3: ax_s5 (add_singleton G x) F_).
+  { destruct (excluded_middle (ax_s5 (add_singleton G x) F_)).
+  - assumption.
+  - contradiction. }
+  apply HG, (mp _ x).
+  - apply deduction_theorem. apply H3. 
+  - apply deduction_theorem in H2. apply (mp _ (Impl (Neg x) F_)).
+    + apply ax_s5_dne.
+    + apply H2.
+Qed.
+
+Lemma inconsistent_consistent_neg (G : Form -> Prop) (x : Form) : 
+  consistent G -> 
+  ~ consistent (add_singleton G (Neg x)) -> consistent (add_singleton G x).
+Proof.
+  intros HG H1 H2. assert (H3: ax_s5 (add_singleton G (Neg x)) F_).
+  { destruct (excluded_middle (ax_s5 (add_singleton G (Neg x)) F_)).
+  - assumption.
+  - contradiction. }
+  apply HG. apply (mp _ (Neg x)).
+  - apply deduction_theorem. apply H3. 
+  - apply deduction_theorem in H2. apply (mp _ (Impl (x) F_)).
+    + apply ax_s5_self_impl.
+    + apply H2.
+Qed.
+
+Lemma consistent_add_or (G : Form -> Prop) (x : Form) :
+  consistent G ->
+  (consistent (add_singleton G x)) \/ (consistent (add_singleton G (Neg x))).
+Proof.
+  intros H0.
+  destruct (excluded_middle (consistent (add_singleton G x))) as [H1|H1].
+  { left. assumption. }
+  right. apply inconsistent_consistent; assumption.
+Qed.
