source/encode.v
@@ -10,3 +10,7 @@ Admitted.
 Lemma decode_encode (n : nat) :
   encode (decode n) = n.
 Admitted.
+
+Lemma encode_decode (x : Form) :
+  decode (encode x) = x.
+Admitted.
