source/maximal.v
@@ -1,0 +1,235 @@
+
+From S5 Require Export consistent.
+From S5 Require Export encode.
+
+Definition insert (G : Form -> Prop) (n : nat) : (Form -> Prop) := 
+  fun g =>
+    let f := decode n in
+    G g \/ (consistent (add_singleton G f) /\ g = f) \/ 
+    (~ consistent (add_singleton G f) /\ g = Neg f).
+
+Lemma insert_consistent (G : Form -> Prop) (n : nat) : 
+  consistent G -> consistent (insert G n).
+Proof.  
+  intros H. unfold insert. pose (f := decode n). fold f.
+  destruct (excluded_middle (consistent (add_singleton G f))) as [Hcon1|Hcon1].
+  - apply (consistent_subset _ (add_singleton G f)). split.
+    + unfold add_singleton. intros x [Hx | [H1 | H1]].
+      * right. assumption.
+      * left. apply H1.
+      * unfold add_singleton in Hcon1. destruct H1. contradiction.
+    + assumption. 
+  - apply (consistent_subset _ (add_singleton G (Neg f))). split.
+    + intros g [H1 | [H2 | H3]].
+      * right. assumption. 
+      * destruct H2 as [H1 H2]. contradiction.
+      * destruct H3 as [H1 H2]. left. assumption.
+    + apply inconsistent_consistent; assumption.
+Qed.
+
+Lemma insert_subset (G : Form -> Prop) (n : nat) : 
+  subset G (insert G n).
+Proof.
+  intros g H. left. assumption.
+Qed.
+
+Fixpoint step (G : Form -> Prop) (n : nat) : (Form -> Prop) :=
+  match n with
+  | 0 => G
+  | S n => insert (step G n) n
+  end.
+
+Lemma step_consistent (G : Form -> Prop) :
+  consistent G -> forall n, consistent (step G n).
+Proof.
+  induction n.
+  - assumption.
+  - simpl. apply insert_consistent, IHn.
+Qed.
+
+Lemma step_maximal (G : Form -> Prop) (x : Form) :
+  consistent G -> step G (S (encode x)) x \/ step G (S (encode x)) (Neg x).
+Proof.
+  intros H0. pose (n := encode x). fold n. assert (H1: decode (encode x) = x).
+  { apply encode_decode. }
+   destruct (excluded_middle (consistent (add_singleton (step G (encode x)) x))) as [H2|H2].
+  - left. simpl. unfold insert. right. left. unfold n. rewrite H1. split.
+    + assumption.
+    + reflexivity.
+  - right. simpl. unfold insert. right. right. unfold n. rewrite H1. split.
+    + assumption.
+    + reflexivity.
+Qed.
+
+Definition big_union (F : nat -> (Form -> Prop)) (x : Form) : Prop :=
+  exists i, (F i) x.
+
+Definition max_consistent_set (G : Form -> Prop) : Form -> Prop :=
+  big_union (step G).
+
+Lemma max_consistent_set_maximal (G : Form -> Prop) (f : Form) :
+  consistent G -> max_consistent_set G f \/ max_consistent_set G (Neg f).
+Proof.
+  intros H0. pose (n := encode f). unfold max_consistent_set, big_union.
+  destruct (step_maximal G f) as [H1|H1].
+  - apply H0.
+  - left. exists (S n). assumption.
+  - right. exists (S n). assumption.
+Qed.
+
+Lemma max_consistent_set_consistent (G : Form -> Prop) :
+  consistent G -> consistent (max_consistent_set G).
+Proof.
+  intros H0 H1. unfold max_consistent_set in H1. remember (big_union (step G)) as G'.
+  induction H1; subst.
+  - unfold big_union in H. destruct H as [n]. pose (m := n - 1).
+    assert (H2: S m = n). { admit. }
+    rewrite <- H2 in H. simpl in H. unfold insert in H.
+Admitted.
+
+Definition max_consistent (G : Form -> Prop) : Prop :=
+  consistent G /\ forall x, (G x \/ G (Neg x)).
+
+Lemma max_consistent_set_correct (G : Form -> Prop) :
+  consistent G -> max_consistent (max_consistent_set G).
+Proof.
+  intros H.
+  unfold max_consistent. split.
+  - apply max_consistent_set_consistent. assumption.
+  - intros f. apply max_consistent_set_maximal. assumption.
+Qed.
+
+Lemma max_consistent_member (G : Form -> Prop) (f : Form) :
+  max_consistent G -> (G f <-> ax_s5 G f).
+Proof.
+  intros H0. split; intros H1.
+  - apply a_0, H1.
+  - unfold max_consistent in H0. destruct H0 as [H2 H3]. specialize (H3 f). destruct H3.
+    + assumption.
+    + exfalso. apply (consistent_xor G f).
+      * assumption.
+      * split.
+        -- assumption.
+        -- apply a_0. assumption.
+Qed.
+
+Lemma max_consistent_subset (G : Form -> Prop) :
+  consistent G -> subset G (max_consistent_set G).
+Proof.
+  intros H0 f H1. unfold max_consistent_set, big_union. pose (n := encode f).
+  exists n. induction n.
+  - unfold step. assumption.
+  - simpl. apply insert_subset. assumption.
+Qed.
+
+Lemma max_consistent_truth (G : Form -> Prop) :
+  consistent G -> max_consistent_set G T_.
+Proof.
+  intros H0. assert (H1: max_consistent (max_consistent_set G)).
+  { apply max_consistent_set_correct, H0. }
+  unfold max_consistent in H1. destruct H1 as [H1 H2]. specialize (H2 T_).
+  destruct H2 as [H2|H2].
+  - assumption.
+  - exfalso. unfold max_consistent_set, big_union in H2. destruct H2 as [n].
+    apply a_0 in H. eapply ax_s5_not_neg_truth, H.
+Qed.
+
+Lemma max_consistent_false (G : Form -> Prop) :
+  consistent G -> ~max_consistent_set G F_.
+Proof.
+  intros H0 H1. assert (H2: max_consistent (max_consistent_set G)).
+  { apply max_consistent_set_correct, H0. }
+  unfold max_consistent in H2. destruct H2 as [H2 H3]. apply H2. apply a_0, H1.
+Qed.
+
+Lemma max_consistent_neg (G : Form -> Prop) (f : Form) :
+  consistent G -> (max_consistent_set G (Neg f) <-> ~max_consistent_set G f).
+Proof.
+  intros H0. assert (H1: max_consistent (max_consistent_set G)).
+  { apply max_consistent_set_correct, H0. }
+  unfold max_consistent in H1. destruct H1 as [H1 H2].
+  split; intros H3.
+  - intros H4. eapply consistent_xor. 
+    + apply H1.
+    + split.
+      * apply max_consistent_member in H4.
+        -- apply H4.
+        -- unfold max_consistent. split; assumption.
+      * apply max_consistent_member in H3.
+        -- apply H3.
+        -- unfold max_consistent. split; assumption.
+  - specialize (H2 f). destruct H2 as [H2|H2].
+    + contradiction.
+    + assumption.
+Qed.
+
+Lemma max_consistent_conj (G : Form -> Prop) (f g : Form) :
+  consistent G ->
+  (max_consistent_set G (Conj f g) <-> max_consistent_set G f /\ max_consistent_set G g).
+Proof.
+  intros H0. assert (H1: max_consistent (max_consistent_set G)).
+  { apply max_consistent_set_correct, H0. }
+  unfold max_consistent in H1. destruct H1 as [H1 H2].
+  split; intros H3.
+  - split.
+    + unfold Conj, Disj in H3.
+Admitted.
+
+Lemma lindenbaum_lemma_1 (G : Form -> Prop) (f : Form) :
+  consistent G -> (ax_s5 G f <-> max_consistent_set G f).
+Proof.
+  intros H0. assert (H1: max_consistent (max_consistent_set G)).
+  { apply max_consistent_set_correct, H0. }
+  unfold max_consistent in H1. destruct H1 as [H2 H3].
+  split; intros H4; specialize (H3 f).
+  - destruct (excluded_middle (max_consistent_set G f)).
+    + assumption.
+    + exfalso. destruct H3 as [H3|H3].
+      * contradiction. 
+      * apply (consistent_xor (max_consistent_set G) f).
+        -- assumption.
+        -- split.
+          ++ apply (ax_s5_subset G (max_consistent_set G)).
+            ** assumption.
+            ** apply max_consistent_subset, H0.
+          ++ apply a_0, H3.
+  - unfold max_consistent_set, big_union in H4. destruct H4 as [n H4]. induction n.
+    + unfold step in H4. apply a_0, H4.
+    + unfold max_consistent_set, big_union in H3. 
+      simpl in H4. unfold insert in H4. destruct H4 as [H4|[H4|H4]].
+      * apply IHn, H4.
+      * destruct H4 as [H4 H5]. rewrite <- H5 in H4. destruct H3 as [H3|H3].
+        -- destruct H3 as [n']. assert (H6: n = n'). admit. rewrite <- H6 in H.
+           apply IHn, H.
+        -- destruct H3 as [n']. assert (H6: n = n'). admit. rewrite <- H6 in H.
+           exfalso. eapply deduce_not_consistent_add_neg_singleton. split.
+          ++ apply (step_consistent G), H0.
+          ++ apply a_0 in H. apply H.
+          ++ admit.
+      * destruct H4 as [H4 H5]. destruct H3 as [H3|H3].
+        -- destruct H3 as [n']. assert (H6: n = n'). admit. rewrite <- H6 in H.
+           apply IHn, H.
+        --
+Admitted.
+
+Lemma lindenbaum_lemma_2 (G : Form -> Prop) (f : Form) :
+  consistent G -> (ax_s5 empty_set f <-> max_consistent_set G f).
+Proof.
+  intros H0. assert (H1: max_consistent (max_consistent_set G)).
+  { apply max_consistent_set_correct, H0. }
+  unfold max_consistent in H1. destruct H1 as [H2 H3].
+  split; intros H4; specialize (H3 f).
+  - destruct (excluded_middle (max_consistent_set G f)).
+    + assumption.
+    + exfalso. destruct H3 as [H3|H3].
+      * contradiction. 
+      * apply (consistent_xor (max_consistent_set G) f).
+        -- assumption.
+        -- split.
+          ++ apply (ax_s5_subset empty_set (max_consistent_set G)).
+            ** assumption.
+            ** apply empty_subset.
+          ++ apply a_0, H3. 
+  - admit.
+Admitted.
+  
